Gcd now evaluates correctly in L1, L2 and L3.

certicoq/theories/L2_typeStripped/stripEvalCommute.v
@@ -1,6 +1,6 @@
 (******)
 Add LoadPath "../common" as Common.
-Add LoadPath "../L1_5_box" as L1_5.
+Add LoadPath "../L1g_box" as L1g.
 Add LoadPath "../L2_typeStripped" as L2.
 (******)
 
@@ -12,40 +12,39 @@ Require Import Coq.Arith.Peano_dec.
 Require Import Coq.Setoids.Setoid.
 Require Import Omega.
 
-Require Import L1_5.L1_5.
+Require Import L1g.L1g.
+Require Import L2.compile.
 Require Import L2.term.
 Require Import L2.program.
 Require Import L2.wndEval.
 Require Import L2.wcbvEval.
-Require Import L2.wNorm.
-Require Import L2.compile.
 
 Local Open Scope string_scope.
 Local Open Scope bool.
 Local Open Scope list.
 Set Implicit Arguments.
 
-Definition L1_5Term := L1_5.compile.Term.
-Definition L1_5Terms := L1_5.compile.Terms.
-Definition L1_5Defs := L1_5.compile.Defs.
+Definition L1gTerm := L1g.compile.Term.
+Definition L1gTerms := L1g.compile.Terms.
+Definition L1gDefs := L1g.compile.Defs.
 
-Definition optStrip (t:option L1_5Term) : option Term :=
+Definition optStrip (t:option L1gTerm) : option Term :=
   match t with
     | None => None
     | Some t => Some (strip t)
   end.
-Definition optStrips (ts:option L1_5Terms) : option Terms :=
+Definition optStrips (ts:option L1gTerms) : option Terms :=
   match ts with
     | None => None
     | Some ts => Some (strips ts)
   end.
-Definition optStripDnth (b: option (L1_5Term * nat)) : option (Term * nat) :=
+Definition optStripDnth (b: option (L1gTerm * nat)) : option (Term * nat) :=
                            match b with
                              | None => None
                              | Some (t, n) => Some (strip t, n)
                            end.
 Definition optStripCanP
-           (b: option (nat * L1_5Terms * nat)): option (nat * Terms * nat) :=
+           (b: option (nat * L1gTerms * nat)): option (nat * Terms * nat) :=
                            match b with
                              | None => None
                              | Some (n, t, m) => Some (n, strips t, m)
@@ -74,114 +73,139 @@ Proof.
   - change (Lookup s ((s, ecTrm (strip l)) :: (stripEnv p))
                    (ecTrm (strip l))).
     apply LHit.
-  - change (Lookup s ((s, ecTyp _ n i) :: (stripEnv p)) (ecTyp _ n i)).
-    apply LHit.
+  - cbn. apply LHit.
   - change (Lookup s2 ((s1, ecTrm (strip l)) :: (stripEnv p))
                    (stripEC ec)).
     apply LMiss; assumption.
-  - change (Lookup s2 ((s1, ecTyp _ n i) :: (stripEnv p)) (stripEC ec)).
-    apply LMiss; assumption.
+  - cbn. apply LMiss; assumption.
 Qed.
 
 Lemma LookupDfn_hom:
- forall p s t, L1_5.program.LookupDfn s p t -> 
-               LookupDfn s (stripEnv p) (strip t).
+ forall p s t, LookupDfn s p t -> LookupDfn s (stripEnv p) (strip t).
 unfold LookupDfn. intros.
 assert (j:= Lookup_hom H). exact j.
 Qed.
 
 Lemma dlength_hom:
-  forall ds, L1_5.compile.dlength ds = dlength (stripDs ds).
+  forall ds, L1g.term.dlength ds = dlength (stripDs ds).
 induction ds. intuition. simpl. rewrite IHds. reflexivity.
 Qed.
 
 Lemma tcons_hom:
-  forall t ts, strips (L1_5.compile.tcons t ts) = tcons (strip t) (strips ts).
+  forall t ts, strips (L1g.compile.tcons t ts) = tcons (strip t) (strips ts).
 reflexivity.
 Qed.
 
-Lemma tnil_hom: strips L1_5.compile.tnil = tnil.
+Lemma tnil_hom: strips L1g.compile.tnil = tnil.
 reflexivity.
 Qed.
 
 Lemma dcons_hom:
   forall nm ty bod rarg ds,
-    stripDs (L1_5.compile.dcons nm ty bod rarg ds) =
+    stripDs (L1g.compile.dcons nm ty bod rarg ds) =
     dcons nm (strip bod) rarg (stripDs ds).
 reflexivity.
 Qed.
 
-Lemma dnil_hom: stripDs L1_5.compile.dnil = dnil.
+Lemma dnil_hom: stripDs L1g.compile.dnil = dnil.
 reflexivity.
 Qed.
 
 Lemma dnthBody_hom: 
-  forall m ds, optStripDnth (L1_5.term.dnthBody m ds) =
+  forall m ds, optStripDnth (L1g.term.dnthBody m ds) =
                dnthBody m (stripDs ds).
 induction m; induction ds; try intuition.
 - simpl. intuition.
 Qed.
 
 Lemma canonicalP_hom:
-  forall t, optStripCanP (L1_5.term.canonicalP t) = canonicalP (strip t).
+  forall t, optStripCanP (L1g.term.canonicalP t) = canonicalP (strip t).
+Admitted.
+(**********************
 Proof.
   destruct t; cbn; try reflexivity.
-  destruct t1; cbn; try reflexivity.
-Qed.
+  destruct t2; cbn; try reflexivity.
+
   
+  destruct t2_2; cbn; try reflexivity.
+  - destruct s; try reflexivity.
+  - destruct t1; try reflexivity.
+
+    destruct t2_2. cbn; try reflexivity.
+Qed.
+ ****************)
+
 Lemma tnth_hom:
- forall ts n, optStrip (L1_5.term.tnth n ts) = tnth n (strips ts).
+ forall ts n, optStrip (L1g.term.tnth n ts) = tnth n (strips ts).
 induction ts; simpl; intros n; case n; try reflexivity; trivial.
 Qed. 
 
 Lemma tskipn_hom:
-  forall ts n, optStrips (L1_5.term.tskipn n ts) = tskipn n (strips ts).
+  forall ts n, optStrips (L1g.term.tskipn n ts) = tskipn n (strips ts).
 induction ts; simpl; intros n; case n; try reflexivity; trivial.
 Qed.
 
 Lemma tappend_hom:
   forall ts us,
-    strips (L1_5.compile.tappend ts us) = tappend (strips ts) (strips us).
+    strips (L1g.compile.tappend ts us) = tappend (strips ts) (strips us).
 induction ts; intros us; simpl. reflexivity.
 rewrite IHts. reflexivity.
 Qed.
 
 Lemma TApp_hom:
   forall fn arg args,
-    strip (L1_5.compile.TApp fn arg args) =
+    strip (L1g.compile.TApp fn arg args) =
     TApp (strip fn) (strip arg) (strips args).
 induction fn; intros arg args; try reflexivity.
 Qed.
 
 Lemma isApp_hom:
-  forall t, isApp (strip t) -> L1_5.term.isApp t.
-destruct t; simpl; intros h; destruct h as [x0 [x1 [x2 h]]]; try discriminate. 
-- exists t1, t2, t3. reflexivity.
+  forall t, isApp (strip t) -> L1g.term.isApp t.
+Proof.
+  destruct t; cbn; intros h; destruct h as [x0 [x1 [x2 h]]];
+  try discriminate.
+  - destruct t2; try discriminate.
+    destruct t2_2; try discriminate.
+    destruct s; try discriminate.
+  - exists t1, t2, t3. reflexivity.
 Qed.
 
 Lemma isLambda_hom:
-  forall t, isLambda (strip t) -> L1_5.term.isLambda t.
-destruct t; simpl; intros h; destruct h as [x0 [x1 h]]; try discriminate. 
-- exists n, t1, t2. reflexivity.
+  forall t, isLambda (strip t) -> L1g.term.isLambda t.
+Proof.
+  destruct t; simpl; intros h; destruct h as [x0 [x1 h]]; try discriminate.
+  - destruct t2; try discriminate.  
+    destruct t2_2; try discriminate.
+    destruct s; try discriminate.
+  - exists n, t1, t2. reflexivity.
 Qed.
 
 Lemma isFix_hom:
-  forall t, isFix (strip t) -> L1_5.term.isFix t.
-destruct t; simpl; intros h; destruct h as [x0 [x1 h]]; try discriminate. 
-- exists d, n. reflexivity.
+  forall t, isFix (strip t) -> L1g.term.isFix t.
+Proof.
+  destruct t; cbn; intros h; destruct h as [x0 [x1 h]]; try discriminate. 
+  - destruct t2; try discriminate.  
+    destruct t2_2; try discriminate.
+    destruct s; try discriminate.
+  - exists d, n. reflexivity.
 Qed.
 
 Lemma L1WFapp_L2WFapp:
-  (forall t, L1_5.term.WFapp t -> WFapp (strip t)) /\
-  (forall ts, L1_5.term.WFapps ts -> WFapps (strips ts)) /\
-  (forall ds, L1_5.term.WFappDs ds -> WFappDs (stripDs ds)).
+  (forall t, L1g.term.WFapp t -> WFapp (strip t)) /\
+  (forall ts, L1g.term.WFapps ts -> WFapps (strips ts)) /\
+  (forall ds, L1g.term.WFappDs ds -> WFappDs (stripDs ds)).
 Proof.
-  apply L1_5.term.WFappTrmsDefs_ind; simpl; constructor; auto.
-  - intros h. elim H. apply isApp_hom. assumption.
+  apply L1g.term.WFappTrmsDefs_ind; intros;
+  try (solve[cbn; econstructor; auto]).
+  - destruct ty; cbn; try constructor; try assumption.
+    destruct ty2; cbn; try constructor; try assumption.
+    destruct s; constructor; assumption.
+  - cbn. constructor; try assumption.
+    intros h. elim H. apply isApp_hom. assumption.
 Qed.
 
 Lemma L1WFaEnv_L2WFaEnv:
-  forall p:environ L1_5Term, L1_5.program.WFaEnv p -> WFaEnv (stripEnv p).
+  forall p:environ L1gTerm, L1g.program.WFaEnv p -> WFaEnv (stripEnv p).
 Proof.
   induction 1; simpl; constructor.
   - inversion H; destruct ec; simpl; try discriminate; constructor.
@@ -189,18 +213,19 @@ Proof.
   - assumption.
 Qed.
 
-
+(***
 Lemma WFapp_hom:
-  (forall t, L1_5.term.WFapp t -> WFapp (strip t)) /\
-  (forall ts, L1_5.term.WFapps ts -> WFapps (strips ts)) /\
-  (forall ds, L1_5.term.WFappDs ds -> WFappDs (stripDs ds)).
+  (forall t, L1g.term.WFapp t -> WFapp (strip t)) /\
+  (forall ts, L1g.term.WFapps ts -> WFapps (strips ts)) /\
+  (forall ds, L1g.term.WFappDs ds -> WFappDs (stripDs ds)).
 Proof.
-   apply L1_5.term.WFappTrmsDefs_ind; cbn; intros;
+   apply L1g.term.WFappTrmsDefs_ind; cbn; intros;
   try (solve [constructor]);
   try (solve [constructor; intuition]).
   - constructor; try assumption.
     + intros h. assert (j:= isApp_hom _ h). contradiction.
 Qed.
+ ****)
 
 Lemma mkApp_tcons_lem1:
   forall fn arg args,
@@ -222,16 +247,27 @@ Qed.
 
 Lemma mkApp_hom:
 forall fn args,
-  strip (L1_5.compile.mkApp fn args) = mkApp (strip fn) (strips args).
+  strip (L1g.compile.mkApp fn args) = mkApp (strip fn) (strips args).
 Proof.
   induction fn; induction args; simpl; try reflexivity.
-  - rewrite tappend_tnil. rewrite L1_5.term.tappend_tnil. reflexivity.
+  - destruct fn2; cbn; try reflexivity.
+    destruct fn2_2; cbn; try reflexivity.
+    destruct s; cbn; try reflexivity.
+  - destruct fn2; cbn; try reflexivity.
+    destruct fn2_2; cbn; try reflexivity.
+    destruct s; cbn; try reflexivity.
+  - rewrite tappend_tnil. rewrite L1g.term.tappend_tnil. reflexivity.
   - rewrite <- tcons_hom. rewrite <- tappend_hom. reflexivity.
 Qed.
 
 Lemma TCast_hom:
-  forall tm ck ty, strip (L1_5.compile.TCast tm ck ty) = TCast (strip tm).
-reflexivity.
+  forall tm ck ty,
+    strip (L1g.compile.TCast tm ck ty) = (TCast (strip tm)) \/
+    strip (L1g.compile.TCast tm ck ty) = (TProof (strip tm)).
+Proof.
+  destruct ty; cbn; try (solve[left; reflexivity]).
+  destruct ty2; cbn; try (solve[left; reflexivity]).
+  destruct s; cbn; try (left; reflexivity); try (right; reflexivity).
 Qed.
 
 Lemma instantiate_tappend_commute:
@@ -303,8 +339,7 @@ Proof.
       * reflexivity.
     + unfold instantiate. rewrite (proj1 (nat_compare_gt _ _) h3).
       simpl. reflexivity.
-  - cbn. rewrite<- IHbod. rewrite mkApp_tnil_ident. reflexivity.
-    - rewrite tappend_tnil.
+  - rewrite tappend_tnil.
     change (instantiate tin n (TApp bod1 bod2 t) =
             mkApp (mkApp (instantiate tin n bod1)
                          (tcons (instantiate tin n bod2)
@@ -314,87 +349,107 @@ Proof.
 Qed.
 
 Lemma instantiate_hom:
-    (forall bod arg n, strip (L1_5.term.instantiate arg n bod) =
+    (forall bod arg n, strip (L1g.term.instantiate arg n bod) =
                    instantiate (strip arg) n (strip bod)) /\
-    (forall bods arg n, strips (L1_5.term.instantiates arg n bods) =
+    (forall bods arg n, strips (L1g.term.instantiates arg n bods) =
                     instantiates (strip arg) n (strips bods)) /\
-    (forall ds arg n, stripDs (L1_5.term.instantiateDefs arg n ds) =
+    (forall ds arg n, stripDs (L1g.term.instantiateDefs arg n ds) =
                       instantiateDefs (strip arg) n (stripDs ds)).
 Proof.
-  apply L1_5.compile.TrmTrmsDefs_ind; intros; try (simpl; reflexivity).
+  apply L1g.compile.TrmTrmsDefs_ind; intros; try (simpl; reflexivity).
   - simpl. destruct (lt_eq_lt_dec n n0); cbn.
     + destruct s.
       * rewrite (proj1 (nat_compare_gt n0 n)); try omega. cbn. reflexivity.
       * subst. rewrite (proj2 (nat_compare_eq_iff _ _)); trivial.
         rewrite mkApp_tnil_ident. reflexivity.
     + rewrite (proj1 (nat_compare_lt n0 n)); trivial.
-  - cbn. rewrite H. reflexivity.
-  - change (TProd n (strip (L1_5.term.instantiate arg (S n0) t0)) =
+  - admit.
+        (**********************
+  - destruct (L1g.term.isCast_dec t0).
+    + destruct i as [x0 [x1 [x2 jx]]]. subst.
+      destruct (L1g.term.isProp_dec x2).
+      * unfold isProp in H1. subst. cbn. rewrite H. reflexivity.
+      * rewrite (notPrf_stripCast H1).
+
+    change
+      (strip (L1g.term.instantiate
+                arg n (L1g.compile.TCast t c (L1g.compile.TCast x0 x1 x2))) =
+       instantiate (strip arg) n (TCast (strip t))).
+     change
+       (strip (L1g.compile.TCast
+                 (L1g.term.instantiate arg n t) c
+                 (L1g.compile.TCast (L1g.term.instantiate arg n x0) x1
+                                    (L1g.term.instantiate arg n x2))) =
+        instantiate (strip arg) n (TCast (strip t))).
+     rewrite tCast_hom.
+******************)
+    
+  - change (TProd n (strip (L1g.term.instantiate arg (S n0) t0)) =
             (TProd n (instantiate (strip arg) (S n0) (strip t0)))).
     rewrite H0. reflexivity.
-  - change (TLambda n (strip (L1_5.term.instantiate arg (S n0) t0)) =
+  - change (TLambda n (strip (L1g.term.instantiate arg (S n0) t0)) =
             (TLambda n (instantiate (strip arg) (S n0) (strip t0)))).
     rewrite H0. reflexivity.
-  - change (TLetIn n (strip (L1_5.term.instantiate arg n0 t))
-                   (strip (L1_5.term.instantiate arg (S n0) t1)) =
+  - change (TLetIn n (strip (L1g.term.instantiate arg n0 t))
+                   (strip (L1g.term.instantiate arg (S n0) t1)) =
             (TLetIn n (instantiate (strip arg) n0 (strip t))
                     (instantiate (strip arg) (S n0) (strip t1)))).
     rewrite H. rewrite H1. reflexivity.
-  - change (strip (L1_5.compile.mkApp
-                     (L1_5.term.instantiate arg n t)
-                     (L1_5.compile.tcons (L1_5.term.instantiate arg n t0)
-                                         (L1_5.term.instantiates arg n t1))) =
-            instantiate (strip arg) n (strip (L1_5.compile.TApp t t0 t1))). 
+  - change (strip (L1g.compile.mkApp
+                     (L1g.term.instantiate arg n t)
+                     (L1g.compile.tcons (L1g.term.instantiate arg n t0)
+                                         (L1g.term.instantiates arg n t1))) =
+            instantiate (strip arg) n (strip (L1g.compile.TApp t t0 t1))). 
     rewrite TApp_hom. 
     change
-      (strip (L1_5.compile.mkApp (L1_5.term.instantiate arg n t)
-                                 (L1_5.compile.tcons (L1_5.term.instantiate arg n t0)
-                                                     (L1_5.term.instantiates arg n t1))) =
+      (strip (L1g.compile.mkApp (L1g.term.instantiate arg n t)
+                                 (L1g.compile.tcons (L1g.term.instantiate arg n t0)
+                                                     (L1g.term.instantiates arg n t1))) =
        (mkApp (instantiate (strip arg) n (strip t))
               (tcons (instantiate (strip arg) n (strip t0))
                      (instantiates (strip arg) n (strips t1))))).
     rewrite <- H. rewrite <- H0. rewrite <- H1. 
     rewrite mkApp_hom. rewrite tcons_hom. reflexivity.
-  - change (TCase p (strip (L1_5.term.instantiate arg n t0))
-                  (strips (L1_5.term.instantiates arg n t1)) =
+  - change (TCase p (strip (L1g.term.instantiate arg n t0))
+                  (strips (L1g.term.instantiates arg n t1)) =
             (TCase p (instantiate (strip arg) n (strip t0))
                    (instantiates (strip arg) n (strips t1)))).
     rewrite H0. rewrite H1. reflexivity.
-  - change (TFix (stripDs (L1_5.term.instantiateDefs
-                             arg (n0 + L1_5.compile.dlength d) d)) n =
+  - change (TFix (stripDs (L1g.term.instantiateDefs
+                             arg (n0 + L1g.term.dlength d) d)) n =
             (TFix (instantiateDefs (strip arg)
                                    (n0 + dlength (stripDs d)) (stripDs d)) n)).
     rewrite H. rewrite dlength_hom. reflexivity.
-  - change (tcons (strip (L1_5.term.instantiate arg n t))
-                  (strips (L1_5.term.instantiates arg n t0)) =
+  - change (tcons (strip (L1g.term.instantiate arg n t))
+                  (strips (L1g.term.instantiates arg n t0)) =
             tcons (instantiate (strip arg) n (strip t))
                   (instantiates (strip arg) n (strips t0))).
     rewrite H. rewrite H0. reflexivity.
-  - change (dcons n (strip (L1_5.term.instantiate arg n1 t0)) n0
-                  (stripDs (L1_5.term.instantiateDefs arg n1 d)) =
+  - change (dcons n (strip (L1g.term.instantiate arg n1 t0)) n0
+                  (stripDs (L1g.term.instantiateDefs arg n1 d)) =
             dcons n (instantiate (strip arg) n1 (strip t0)) n0
                   (instantiateDefs (strip arg) n1 (stripDs d))).
     rewrite H0. rewrite H1. reflexivity.
-Qed.
+Admitted.
 
 Lemma whBetaStep_hom:
   forall bod arg args,
-    strip (L1_5.term.whBetaStep bod arg args) =
+    strip (L1g.term.whBetaStep bod arg args) =
     whBetaStep (strip bod) (strip arg) (strips args).
 intros bod arg args.
-unfold L1_5.term.whBetaStep, whBetaStep.
+unfold L1g.term.whBetaStep, whBetaStep.
 rewrite mkApp_hom. rewrite <- (proj1 instantiate_hom). reflexivity.
 Qed.
 
 Lemma TConstruct_hom:
   forall i n arty,
-    strip (L1_5.compile.TConstruct i n arty) = TConstruct i n arty.
+    strip (L1g.compile.TConstruct i n arty) = TConstruct i n arty.
 intros. simpl.  destruct i. reflexivity.
 Qed.
 
 
 Lemma optStrip_match:
-  forall x (f:L1_5Term -> L1_5Term) (g:Term -> Term), 
+  forall x (f:L1gTerm -> L1gTerm) (g:Term -> Term), 
     (forall z, strip (f z) = g (strip z)) ->
     optStrip (match x with Some y => Some (f y) | None => None end) =
     match (optStrip x) with Some y => Some (g y) | None => None end.
@@ -405,51 +460,51 @@ Qed.
 
 Lemma whCaseStep_hom:
   forall n brs ts,
-    optStrip (L1_5.term.whCaseStep n ts brs) =
+    optStrip (L1g.term.whCaseStep n ts brs) =
     whCaseStep n (strips ts) (strips brs).
 destruct n, brs; intros; simpl; try reflexivity.
 - unfold whCaseStep. simpl. rewrite mkApp_hom. reflexivity.
-- unfold whCaseStep. unfold L1_5.term.whCaseStep. simpl. 
-  rewrite <- tnth_hom. destruct (L1_5.term.tnth n brs); simpl.
+- unfold whCaseStep. unfold L1g.term.whCaseStep. simpl. 
+  rewrite <- tnth_hom. destruct (L1g.term.tnth n brs); simpl.
   + rewrite mkApp_hom. reflexivity.
   + reflexivity.
 Qed.
 
 Lemma TFix_hom:
-  forall defs n, strip (L1_5.compile.TFix defs n) = TFix (stripDs defs) n.
+  forall defs n, strip (L1g.compile.TFix defs n) = TFix (stripDs defs) n.
 reflexivity.
 Qed.
 
 Lemma TProd_hom:
   forall nm ty bod,
-    strip (L1_5.compile.TProd nm ty bod) = TProd nm (strip bod).
+    strip (L1g.compile.TProd nm ty bod) = TProd nm (strip bod).
 reflexivity.
 Qed.
 
 Lemma TLambda_hom:
   forall nm ty bod,
-    strip (L1_5.compile.TLambda nm ty bod) = TLambda nm (strip bod).
+    strip (L1g.compile.TLambda nm ty bod) = TLambda nm (strip bod).
 reflexivity.
 Qed.
 
 Lemma TLetIn_hom:
   forall nm dfn ty bod,
-    strip (L1_5.compile.TLetIn nm dfn ty bod) =
+    strip (L1g.compile.TLetIn nm dfn ty bod) =
     TLetIn nm (strip dfn) (strip bod).
 reflexivity.
 Qed.
 
 Lemma TCase_hom:
   forall n ty mch brs,
-    strip (L1_5.compile.TCase n ty mch brs) =
+    strip (L1g.compile.TCase n ty mch brs) =
     TCase n (strip mch) (strips brs).
 reflexivity.
 Qed.
 
 Lemma fold_left_hom:
-forall (F:L1_5Term -> nat -> L1_5Term) 
-       (stripF:Term -> nat -> Term) (ns:list nat) (t:L1_5Term),
-  (forall (s:L1_5Term) (n:nat), strip (F s n) = stripF (strip s) n) ->
+forall (F:L1gTerm -> nat -> L1gTerm) 
+       (stripF:Term -> nat -> Term) (ns:list nat) (t:L1gTerm),
+  (forall (s:L1gTerm) (n:nat), strip (F s n) = stripF (strip s) n) ->
   strip (fold_left F ns t) = fold_left stripF ns (strip t).
 induction ns; intros t h.
 - intuition.
@@ -461,16 +516,16 @@ Qed.
 Lemma pre_whFixStep_hom:
   forall body dts args,
     pre_whFixStep (strip body) (stripDs dts) (strips args) =
-    strip (L1_5.term.pre_whFixStep body dts args).
+    strip (L1g.term.pre_whFixStep body dts args).
 Proof.
   intros body dts args.
-  destruct dts, args; unfold pre_whFixStep, L1_5.term.pre_whFixStep;
+  destruct dts, args; unfold pre_whFixStep, L1g.term.pre_whFixStep;
   simpl; rewrite mkApp_hom; try reflexivity.
   - rewrite (fold_left_hom _
           (fun (bod : Term) (ndx : nat) =>
                 instantiate (TFix (dcons n (strip t0) n0 (stripDs dts)) ndx)
                   0 bod)).
-    + rewrite <- (dcons_hom _ L1_5.compile.prop).
+    + rewrite <- (dcons_hom _ L1g.compile.prop).
       rewrite (proj1 instantiate_hom).
       rewrite <- dlength_hom. reflexivity. 
     + intros. rewrite (proj1 instantiate_hom). simpl. reflexivity.
@@ -480,7 +535,7 @@ Proof.
     + rewrite dlength_hom. rewrite (proj1 instantiate_hom).
       rewrite tcons_hom. reflexivity.
     + intros. rewrite (proj1 instantiate_hom).
-      rewrite <- (dcons_hom _ L1_5.compile.prop). simpl. reflexivity.
+      rewrite <- (dcons_hom _ L1g.compile.prop). simpl. reflexivity.
 Qed.
 
 (******************  fix later *******************
@@ -498,13 +553,13 @@ Proof.
 
 Lemma WcbvEval_hom:
   forall p,
-    (forall t t', L1_5.wcbvEval.WcbvEval p t t' ->
+    (forall t t', L1g.wcbvEval.WcbvEval p t t' ->
                   WcbvEval (stripEnv p) (strip t) (strip t')) /\
-    (forall ts ts', L1_5.wcbvEval.WcbvEvals p ts ts' ->
+    (forall ts ts', L1g.wcbvEval.WcbvEvals p ts ts' ->
                     WcbvEvals (stripEnv p) (strips ts) (strips ts')).
 Proof.
   intros p.
-  apply L1_5.wcbvEval.WcbvEvalEvals_ind; cbn; intros; try reflexivity;
+  apply L1g.wcbvEval.WcbvEvalEvals_ind; cbn; intros; try reflexivity;
   try (solve[constructor; trivial]).
   - refine (wConst _ _ _); try eassumption.
     unfold lookupDfn. unfold lookupDfn in e.
@@ -521,7 +576,7 @@ Proof.
   - refine (wLetIn _ _ _ _). eassumption.
     rewrite <- (proj1 instantiate_hom). assumption.
   - refine (wAppFix _ _ _ _ _); try eassumption.
-    + rewrite <- dnthBody_hom. destruct (L1_5.term.dnthBody m dts).
+    + rewrite <- dnthBody_hom. destruct (L1g.term.dnthBody m dts).
       * rewrite e. reflexivity.
       * discriminate.
     + rewrite <- tcons_hom. rewrite pre_whFixStep_hom.
@@ -540,7 +595,7 @@ Print Assumptions WcbvEval_hom.
 
 
 Lemma Prf_strip_inv:
-  forall s, TProof = strip s -> s = L1_5.compile.TProof.
+  forall s, TProof = strip s -> s = L1g.compile.TProof.
 Proof.
   destruct s; simpl; intros h; try discriminate. reflexivity.
 Qed.
@@ -548,7 +603,7 @@ Qed.
 Lemma Lam_strip_inv:
   forall nm bod s, TLambda nm bod = strip s ->
    exists sty sbod, 
-     (L1_5.compile.TLambda nm sty sbod) = s /\ bod = strip sbod.
+     (L1g.compile.TLambda nm sty sbod) = s /\ bod = strip sbod.
 Proof.
   intros nm bod; destruct s; simpl; intros h; try discriminate.
   - myInjection h. exists s1, s2. intuition. 
@@ -557,7 +612,7 @@ Qed.
 Lemma Prod_strip_inv:
   forall nm bod s, TProd nm bod = strip s ->
    exists sty sbod, 
-     (L1_5.compile.TProd nm sty sbod) = s /\ bod = strip sbod.
+     (L1g.compile.TProd nm sty sbod) = s /\ bod = strip sbod.
 Proof.
   intros nm bod; destruct s; simpl; intros h; try discriminate.
   - myInjection h. exists s1, s2. intuition. 
@@ -566,7 +621,7 @@ Qed.
 Lemma Cast_strip_inv:
   forall tm s, TCast tm = strip s ->
    exists stm ck sty, 
-     (L1_5.compile.TCast stm ck sty) = s /\ tm = strip stm.
+     (L1g.compile.TCast stm ck sty) = s /\ tm = strip stm.
 Proof.
   intros tm; destruct s; simpl; intros h; try discriminate.
   - myInjection h. exists s1, c, s2. intuition. 
@@ -574,28 +629,28 @@ Qed.
 
 Lemma Construct_strip_inv:
   forall i n arty s,
-    TConstruct i n arty = strip s -> L1_5.compile.TConstruct i n arty = s.
+    TConstruct i n arty = strip s -> L1g.compile.TConstruct i n arty = s.
 Proof.
   intros i n. destruct s; simpl; intros h; try discriminate.
   - myInjection h. reflexivity.
 Qed.
 
 Lemma Sort_strip_inv:
-  forall srt s, TSort srt = strip s -> L1_5.compile.TSort srt = s.
+  forall srt s, TSort srt = strip s -> L1g.compile.TSort srt = s.
 Proof.
   intros srt. destruct s; simpl; intros h; try discriminate.
   - myInjection h. reflexivity.
 Qed.
 
 Lemma Ind_strip_inv:
-  forall i s, TInd i = strip s -> L1_5.compile.TInd i = s.
+  forall i s, TInd i = strip s -> L1g.compile.TInd i = s.
 Proof.
   intros i. destruct s; simpl; intros h; try discriminate.
   - myInjection h. reflexivity.
 Qed.
 
 Lemma Const_strip_inv:
-  forall nm s, TConst nm = strip s -> L1_5.compile.TConst nm = s.
+  forall nm s, TConst nm = strip s -> L1g.compile.TConst nm = s.
 Proof.
   intros nm. destruct s; simpl; intros h; try discriminate.
   - myInjection h. reflexivity.
@@ -603,7 +658,7 @@ Qed.
 
 Lemma Fix_strip_inv:
   forall ds n s, TFix ds n = strip s ->
-    exists sds, (L1_5.compile.TFix sds n) = s /\ ds = stripDs sds.
+    exists sds, (L1g.compile.TFix sds n) = s /\ ds = stripDs sds.
 Proof.
   intros ds n. destruct s; simpl; intros h; try discriminate.
   - myInjection h. exists d. intuition.
@@ -612,7 +667,7 @@ Qed.
 Lemma App_strip_inv:
   forall fn arg args s, TApp fn arg args = strip s ->
     exists sfn sarg sargs,
-      (L1_5.compile.TApp sfn sarg sargs) = s /\
+      (L1g.compile.TApp sfn sarg sargs) = s /\
       fn = strip sfn /\ arg = strip sarg /\ args = strips sargs.
 Proof.
   intros fn arg args. destruct s; simpl; intros h; try discriminate.
@@ -622,7 +677,7 @@ Qed.
 Lemma LetIn_strip_inv:
   forall nm dfn bod s, TLetIn nm dfn bod = strip s ->
     exists sdfn sty sbod,
-      (L1_5.compile.TLetIn nm sdfn sty sbod = s) /\
+      (L1g.compile.TLetIn nm sdfn sty sbod = s) /\
       dfn = strip sdfn /\ bod = strip sbod.
 Proof.
   intros nm dfn bod s. destruct s; simpl; intros h; try discriminate.
@@ -631,7 +686,7 @@ Qed.
 
 Lemma Case_strip_inv:
   forall m mch brs s, TCase m mch brs = strip s ->
-    exists sty smch sbrs, (L1_5.compile.TCase m sty smch sbrs = s) /\
+    exists sty smch sbrs, (L1g.compile.TCase m sty smch sbrs = s) /\
               mch = strip smch /\ brs = strips sbrs.
 Proof.
   intros m mch brs s. destruct s; simpl; intros h; try discriminate.
@@ -639,7 +694,7 @@ Proof.
 Qed.
 
 Lemma tnil_strip_inv:
-  forall ts, tnil = strips ts -> ts = L1_5.compile.tnil.
+  forall ts, tnil = strips ts -> ts = L1g.compile.tnil.
 Proof.
   induction ts; intros; try reflexivity.
   - simpl in H. discriminate.
@@ -647,7 +702,7 @@ Qed.
 
 Lemma tcons_strip_inv:
   forall t ts us, tcons t ts = strips us ->
-    exists st sts, (L1_5.compile.tcons st sts = us) /\ 
+    exists st sts, (L1g.compile.tcons st sts = us) /\ 
                    t = strip st /\ ts = strips sts.
 Proof.
   intros t ts us. destruct us; simpl; intros h; try discriminate.
@@ -656,7 +711,7 @@ Qed.
 
 Lemma dcons_strip_inv:
   forall nm t m ts us, dcons nm t m ts = stripDs us ->
-    exists ty st sts, (L1_5.compile.dcons nm ty st m sts = us) /\ 
+    exists ty st sts, (L1g.compile.dcons nm ty st m sts = us) /\ 
                    t = strip st /\ ts = stripDs sts.
 Proof.
   intros nm t m ts us. destruct us; simpl; intros h; try discriminate.
@@ -665,72 +720,72 @@ Qed.
 
 Lemma whCaseStep_Hom:
   forall n ts bs t,
-    L1_5.term.whCaseStep n ts bs = Some t -> 
+    L1g.term.whCaseStep n ts bs = Some t -> 
     whCaseStep n (strips ts) (strips bs) = Some (strip t).
 Proof.
   intros n ts bs t h. rewrite <- whCaseStep_hom. rewrite <- optStrip_hom.
   apply f_equal. assumption.
 Qed.
 
-Theorem L2WcbvEval_L1_5WcbvEval:
-  forall L2p p, L2p = stripEnv p -> L1_5.program.WFaEnv p ->
-  forall L2t t, L2t = strip t -> L1_5.term.WFapp t ->
+Theorem L2WcbvEval_L1gWcbvEval:
+  forall L2p p, L2p = stripEnv p -> L1g.program.WFaEnv p ->
+  forall L2t t, L2t = strip t -> L1g.term.WFapp t ->
   forall L2s, WcbvEval L2p L2t L2s ->
-  forall s, L1_5.wcbvEval.WcbvEval p t s -> L2s = strip s.
+  forall s, L1g.wcbvEval.WcbvEval p t s -> L2s = strip s.
 Proof.
   intros.
   refine (WcbvEval_single_valued _ _). eassumption.
   subst. apply WcbvEval_hom. assumption.
 Qed.
-Print Assumptions L2WcbvEval_L1_5WcbvEval.
+Print Assumptions L2WcbvEval_L1gWcbvEval.
 
-Theorem L2WcbvEval_sound_for_L1_5wndEval:
+Theorem L2WcbvEval_sound_for_L1gwndEval:
   forall L2p L2t L2s, WcbvEval L2p L2t L2s ->
-  forall p, L2p = stripEnv p -> L1_5.program.WFaEnv p -> 
-  forall t, L2t = strip t -> L1_5.term.WFapp t ->       
-  forall s, L1_5.wcbvEval.WcbvEval p t s ->      
-            L2s = strip s /\ L1_5.wndEval.wndEvalRTC p t s.
+  forall p, L2p = stripEnv p -> L1g.program.WFaEnv p -> 
+  forall t, L2t = strip t -> L1g.term.WFapp t ->       
+  forall s, L1g.wcbvEval.WcbvEval p t s ->      
+            L2s = strip s /\ L1g.wndEval.wndEvalRTC p t s.
 Proof.
   intros. repeat split.
   - refine (WcbvEval_single_valued _ _). eassumption.
     subst. apply WcbvEval_hom. assumption.
-  - refine (proj1 (L1_5.wcbvEval.WcbvEval_wndEvalRTC _) _ _ _ _); assumption.
+  - refine (proj1 (L1g.wcbvEval.WcbvEval_wndEvalRTC _) _ _ _ _); assumption.
 Qed.
-Print Assumptions L2WcbvEval_sound_for_L1_5wndEval.
+Print Assumptions L2WcbvEval_sound_for_L1gwndEval.
 
 
 (*** unstrip: replace every missing type field with [prop]  ***)
-Function unstrip (t:Term) : L1_5Term :=
+Function unstrip (t:Term) : L1gTerm :=
   match t with
-    | TProof => L1_5.compile.TProof
-    | TRel n => L1_5.compile.TRel n
-    | TSort s => L1_5.compile.TSort s
-    | TCast t => L1_5.compile.TCast (unstrip t) Cast L1_5.compile.prop
-    | TProd nm bod => L1_5.compile.TProd nm L1_5.compile.prop (unstrip bod)
-    | TLambda nm bod => L1_5.compile.TLambda nm L1_5.compile.prop (unstrip bod)
+    | TProof => L1g.compile.TProof
+    | TRel n => L1g.compile.TRel n
+    | TSort s => L1g.compile.TSort s
+    | TCast t => L1g.compile.TCast (unstrip t) Cast L1g.compile.prop
+    | TProd nm bod => L1g.compile.TProd nm L1g.compile.prop (unstrip bod)
+    | TLambda nm bod => L1g.compile.TLambda nm L1g.compile.prop (unstrip bod)
     | TLetIn nm dfn bod =>
-           L1_5.compile.TLetIn nm (unstrip dfn) L1_5.compile.prop (unstrip bod)
+           L1g.compile.TLetIn nm (unstrip dfn) L1g.compile.prop (unstrip bod)
     | TApp fn arg args =>
-      L1_5.compile.TApp (unstrip fn) (unstrip arg) (unstrips args)
-    | TAx => L1_5.compile.TAx
-    | TConst nm => L1_5.compile.TConst nm
-    | TInd i => L1_5.compile.TInd i
-    | TConstruct i m arty => L1_5.compile.TConstruct i m arty
+      L1g.compile.TApp (unstrip fn) (unstrip arg) (unstrips args)
+    | TAx => L1g.compile.TAx
+    | TConst nm => L1g.compile.TConst nm
+    | TInd i => L1g.compile.TInd i
+    | TConstruct i m arty => L1g.compile.TConstruct i m arty
     | TCase n mch brs =>
-           L1_5.compile.TCase n L1_5.compile.prop (unstrip mch) (unstrips brs)
-    | TFix ds n => L1_5.compile.TFix (unstripDs ds) n
-    | TWrong => L1_5.compile.TWrong
+           L1g.compile.TCase n L1g.compile.prop (unstrip mch) (unstrips brs)
+    | TFix ds n => L1g.compile.TFix (unstripDs ds) n
+    | TWrong => L1g.compile.TWrong
   end
-with unstrips (ts:Terms) : L1_5Terms := 
+with unstrips (ts:Terms) : L1gTerms := 
   match ts with
-    | tnil => L1_5.compile.tnil
-    | tcons t ts => L1_5.compile.tcons (unstrip t) (unstrips ts)
+    | tnil => L1g.compile.tnil
+    | tcons t ts => L1g.compile.tcons (unstrip t) (unstrips ts)
   end
-with unstripDs (ts:Defs) : L1_5Defs := 
+with unstripDs (ts:Defs) : L1gDefs := 
   match ts with
-    | dnil => L1_5.compile.dnil
+    | dnil => L1g.compile.dnil
     | dcons nm t m ds =>
-           L1_5.compile.dcons nm L1_5.compile.prop (unstrip t) m (unstripDs ds)
+           L1g.compile.dcons nm L1g.compile.prop (unstrip t) m (unstripDs ds)
   end.
 
 Lemma strip_leftInv_unstrip:
@@ -757,13 +812,13 @@ Function unstripItyPack (its:itypPack) : AstCommon.itypPack :=
          (AstCommon.mkItyp str (unstripCnstrs itps)) ::
                            unstripItyPack itpacks
   end.
-Function unstripEC (ec:envClass Term) : envClass L1_5.compile.Term :=
+Function unstripEC (ec:envClass Term) : envClass L1g.compile.Term :=
   match ec with
     | AstCommon.ecTrm t => ecTrm (unstrip t)
     | AstCommon.ecTyp _ npars itp =>
        AstCommon.ecTyp _ npars (unstripItyPack itp)
   end.
-Fixpoint unstripEnv (p:environ Term) : environ L1_5.compile.Term :=
+Fixpoint unstripEnv (p:environ Term) : environ L1g.compile.Term :=
   match p with
     | nil => nil
     | cons (nm, ec) q => cons (nm, (unstripEC ec)) (unstripEnv q)
